Update block_number link and simulate to v103 (#874)
Merge BLOCK_NUMBER v103 InstructionContext and Host::block_number update.

RocqOfRust/revm/revm_context_interface/links/host.v
@@ -9,6 +9,7 @@ Require Import core.links.option.
 Require Import core.links.result.
 Require Import revm.revm_context_interface.links.cfg.
 Require Import revm.revm_context_interface.links.block.
+Require Import revm.revm_context_interface.host.
 Require Import revm.revm_context_interface.links.journaled_state.
 Require Import revm.revm_context_interface.links.transaction.
 Require Import ruint.links.lib.
@@ -297,6 +298,7 @@ Export (hints) SelfDestructResult.
 pub trait Host: TransactionGetter + BlockGetter + CfgGetter {
     fn load_account_delegated(&mut self, address: Address) -> Option<AccountLoad>;
     fn block_hash(&mut self, number: u64) -> Option<B256>;
+    fn block_number(&self) -> U256;
     fn balance(&mut self, address: Address) -> Option<StateLoad<U256>>;
     fn code(&mut self, address: Address) -> Option<Eip7702CodeLoad<Bytes>>;
     fn code_hash(&mut self, address: Address) -> Option<Eip7702CodeLoad<B256>>;
@@ -384,6 +386,14 @@ Module Host.
     block_hash_is_method :: IsTraitMethod.C (trait Self) "block_hash" block_hash;
     run_block_hash (self : '&mut Self) (number : u64) ::
       Run.Trait block_hash [] [] [ φ self; φ number ] (option aliases.B256.t);
+  }.
+
+  (* fn block_number(&self) -> U256; *)
+  Class Method_block_number (Self : Set) `{Link Self} : Set := {
+    block_number : PolymorphicFunction.t;
+    block_number_is_method :: IsTraitMethod.C (trait Self) "block_number" block_number;
+    run_block_number (self : '& Self) ::
+      Run.Trait block_number [] [] [ φ self ] aliases.U256.t;
   }.
 
   (* fn balance(&mut self, address: Address) -> Option<StateLoad<U256>>; *)
@@ -490,6 +500,7 @@ Module Host.
     run_CfgGetter_for_Self :: CfgGetter.Run Self (Types.to_CfgGetter_types types);
     method_load_account_delegated :: Method_load_account_delegated Self;
     method_block_hash :: Method_block_hash Self;
+    method_block_number :: Method_block_number Self;
     method_balance :: Method_balance Self;
     method_code :: Method_code Self;
     method_code_hash :: Method_code_hash Self;
@@ -502,3 +513,23 @@ Module Host.
   }.
 End Host.
 Export (hints) Host.
+
+Module Impl_Host_for_RefMut.
+  Instance method_block_number
+      (Self : Set) `{Link Self}
+      (method_block_number : Host.Method_block_number Self) :
+    Host.Method_block_number ('&mut Self).
+  Proof.
+    unshelve econstructor.
+    - exact (host.underscore.Impl_revm_context_interface_host_Host_where_revm_context_interface_host_Host_T_where_core_marker_Sized_T_for_ref_mut_T.block_number (Φ Self)).
+    - constructor.
+      econstructor.
+      + apply host.underscore.Impl_revm_context_interface_host_Host_where_revm_context_interface_host_Host_T_where_core_marker_Sized_T_for_ref_mut_T.Implements.
+      + reflexivity.
+    - intros self.
+      constructor.
+      destruct method_block_number.
+      run_symbolic.
+  Defined.
+End Impl_Host_for_RefMut.
+Export (hints) Impl_Host_for_RefMut.
